<?xml version="1.0"?>
<rdf:RDF xmlns="http://purl.obolibrary.org/obo/cpo#"
     xml:base="http://purl.obolibrary.org/obo/cpo"
     xmlns:rdf="http://www.w3.org/1999/02/22-rdf-syntax-ns#"
     xmlns:owl="http://www.w3.org/2002/07/owl#"
     xmlns:xml="http://www.w3.org/XML/1998/namespace"
     xmlns:xsd="http://www.w3.org/2001/XMLSchema#"
     xmlns:rdfs="http://www.w3.org/2000/01/rdf-schema#"
     xmlns:obo="http://purl.obolibrary.org/obo/"
     xmlns:foaf="http://xmlns.com/foaf/0.1/"
     xmlns:dc="http://purl.org/dc/elements/1.1/">
    <owl:Ontology rdf:about="http://purl.obolibrary.org/obo/cpo">
        <owl:imports rdf:resource="http://purl.obolibrary.org/obo/bfo/2.0/bfo.owl"/>
        <dc:contributor>Cooper Stansbury</dc:contributor>
        <dc:contributor>John Rincon</dc:contributor>
        <owl:versionInfo>0.0.1</owl:versionInfo>
        <dc:contributor>Colin Gross</dc:contributor>
        <dc:contributor>Zach Landis-Lewis</dc:contributor>
        <obo:IAO_0000232>This ontology has been designed to conform to BFO and OBO standards and stands in reference to the following works:

Lewis, Cara C., Predrag Klasnja, Byron J. Powell, Aaron R. Lyon, Leah Tuzzio, Salene Jones, Callie Walsh-Bailey, and Bryan Weiner. “From Classification to Causality: Advancing Understanding of Mechanisms of Change in Implementation Science.” Frontiers in Public Health 6 (2018). https://doi.org/10.3389/fpubh.2018.00136.

Mazza, Danielle, Phillip Bairstow, Heather Buchan, Samantha Paubrey Chakraborty, Oliver Van Hecke, Cathy Grech, and Ilkka Kunnamo. “Refining a Taxonomy for Guideline Implementation: Results of an Exercise in Abstract Classification.” Implementation Science 8 (March 15, 2013): 32. https://doi.org/10.1186/1748-5908-8-32.

Michie, Susan, Stefanie Ashford, Falko F. Sniehotta, Stephan U. Dombrowski, Alex Bishop, and David P. French. “A Refined Taxonomy of Behaviour Change Techniques to Help People Change Their Physical Activity and Healthy Eating Behaviours: The CALO-RE Taxonomy.” Psychology &amp; Health 26, no. 11 (November 1, 2011): 1479–98. https://doi.org/10.1080/08870446.2010.540664.

More publication citations can be found at the annotation property level for the interested reader.</obo:IAO_0000232>
        <dc:license>need to insert license</dc:license>
    </owl:Ontology>
    


    <!-- 
    ///////////////////////////////////////////////////////////////////////////////////////
    //
    // Classes
    //
    ///////////////////////////////////////////////////////////////////////////////////////
     -->

    


    <!-- http://purl.obolibrary.org/obo/cpo#cpo_0000001 -->

    <owl:Class rdf:about="http://purl.obolibrary.org/obo/cpo#cpo_0000001">
        <rdfs:subClassOf rdf:resource="http://purl.obolibrary.org/obo/cpo#cpo_0000004"/>
        <obo:IAO_0000115>a process or event through which an implemnentation strategy operates to affect implementation outcomes</obo:IAO_0000115>
        <obo:IAO_0000116>this definition needs work. it is unclear how the authors of the cited source intend the relationship between moderators and mediators, given that they are not both defined as subclasses with a common parent.</obo:IAO_0000116>
        <obo:IAO_0000119>Lewis CC, Klasnja P, Powell BJ, Lyon AR, Tuzzio L, Jones S, et al. From Classification to Causality: Advancing Understanding of Mechanisms of Change in Implementation Science. Front Public Health [Internet]. 2018 [cited 2018 Jun 6];6. Available from: https://www.frontiersin.org/articles/10.3389/fpubh.2018.00136/full</obo:IAO_0000119>
        <rdfs:label xml:lang="en">mechanism</rdfs:label>
    </owl:Class>
    


    <!-- http://purl.obolibrary.org/obo/cpo#cpo_0000002 -->

    <owl:Class rdf:about="http://purl.obolibrary.org/obo/cpo#cpo_0000002">
        <rdfs:subClassOf rdf:resource="http://purl.obolibrary.org/obo/BFO_0000031"/>
        <obo:IAO_0000115>a factor that is necessary in order for an implementation mechanism or implementation outcome to be activated</obo:IAO_0000115>
        <obo:IAO_0000119>Lewis CC, Klasnja P, Powell BJ, Lyon AR, Tuzzio L, Jones S, et al. From Classification to Causality: Advancing Understanding of Mechanisms of Change in Implementation Science. Front Public Health [Internet]. 2018 [cited 2018 Jun 6];6. Available from: https://www.frontiersin.org/articles/10.3389/fpubh.2018.00136/full</obo:IAO_0000119>
        <rdfs:label xml:lang="en">precondition</rdfs:label>
    </owl:Class>
    


    <!-- http://purl.obolibrary.org/obo/cpo#cpo_0000003 -->

    <owl:Class rdf:about="http://purl.obolibrary.org/obo/cpo#cpo_0000003">
        <rdfs:subClassOf rdf:resource="http://purl.obolibrary.org/obo/BFO_0000031"/>
        <obo:IAO_0000115>a factor that enables or hinders the implementation strategy from eliciting the desired effect</obo:IAO_0000115>
        <obo:IAO_0000116>Also commonly referred to as “barriers” and “facilitators”</obo:IAO_0000116>
        <obo:IAO_0000119>Lewis CC, Klasnja P, Powell BJ, Lyon AR, Tuzzio L, Jones S, et al. From Classification to Causality: Advancing Understanding of Mechanisms of Change in Implementation Science. Front Public Health [Internet]. 2018 [cited 2018 Jun 6];6. Available from: https://www.frontiersin.org/articles/10.3389/fpubh.2018.00136/full</obo:IAO_0000119>
        <rdfs:label xml:lang="en">determinant</rdfs:label>
    </owl:Class>
    


    <!-- http://purl.obolibrary.org/obo/cpo#cpo_0000004 -->

    <owl:Class rdf:about="http://purl.obolibrary.org/obo/cpo#cpo_0000004">
        <rdfs:subClassOf rdf:resource="http://purl.obolibrary.org/obo/BFO_0000015"/>
        <obo:IAO_0000115>an intervening process that affects for the relationship between the implementation strategy and the implementation outcome</obo:IAO_0000115>
        <obo:IAO_0000119>Lewis CC, Klasnja P, Powell BJ, Lyon AR, Tuzzio L, Jones S, et al. From Classification to Causality: Advancing Understanding of Mechanisms of Change in Implementation Science. Front Public Health [Internet]. 2018 [cited 2018 Jun 6];6. Available from: https://www.frontiersin.org/articles/10.3389/fpubh.2018.00136/full</obo:IAO_0000119>
        <rdfs:label xml:lang="en">mediator</rdfs:label>
    </owl:Class>
    


    <!-- http://purl.obolibrary.org/obo/cpo#cpo_0000005 -->

    <owl:Class rdf:about="http://purl.obolibrary.org/obo/cpo#cpo_0000005">
        <rdfs:subClassOf rdf:resource="http://purl.obolibrary.org/obo/BFO_0000015"/>
        <obo:IAO_0000115>a factor that affects the level of influence of an implementation strategy</obo:IAO_0000115>
        <obo:IAO_0000116>moderators functionally &apos;act&apos; on mechanisms, but do not prevent or require mechanisms to &apos;fire.&apos;</obo:IAO_0000116>
        <obo:IAO_0000119>Lewis CC, Klasnja P, Powell BJ, Lyon AR, Tuzzio L, Jones S, et al. From Classification to Causality: Advancing Understanding of Mechanisms of Change in Implementation Science. Front Public Health [Internet]. 2018 [cited 2018 Jun 6];6. Available from: https://www.frontiersin.org/articles/10.3389/fpubh.2018.00136/full</obo:IAO_0000119>
        <rdfs:label xml:lang="en">moderator</rdfs:label>
    </owl:Class>
    


    <!-- http://purl.obolibrary.org/obo/cpo#cpo_0000006 -->

    <owl:Class rdf:about="http://purl.obolibrary.org/obo/cpo#cpo_0000006">
        <rdfs:subClassOf rdf:resource="http://purl.obolibrary.org/obo/cpo#cpo_0000016"/>
        <obo:IAO_0000115>the product of the implementation strategy that is realized because of its specific mechanism of action, the most immediate, observable outcome in the causal pathway</obo:IAO_0000115>
        <obo:IAO_0000119>Lewis et al., “From Classification to Causality.”</obo:IAO_0000119>
        <rdfs:label xml:lang="en">proximal outcome</rdfs:label>
    </owl:Class>
    


    <!-- http://purl.obolibrary.org/obo/cpo#cpo_0000007 -->

    <owl:Class rdf:about="http://purl.obolibrary.org/obo/cpo#cpo_0000007">
        <rdfs:subClassOf rdf:resource="http://purl.obolibrary.org/obo/cpo#cpo_0000016"/>
        <obo:IAO_0000115>the outcome that the implementation processes is ultimately intended to achieve, not the most immediate outcome in the causal pathway</obo:IAO_0000115>
        <obo:IAO_0000119>Lewis et al., “From Classification to Causality.”</obo:IAO_0000119>
        <rdfs:label xml:lang="en">distal outcome</rdfs:label>
    </owl:Class>
    


    <!-- http://purl.obolibrary.org/obo/cpo#cpo_0000008 -->

    <owl:Class rdf:about="http://purl.obolibrary.org/obo/cpo#cpo_0000008">
        <rdfs:subClassOf rdf:resource="http://purl.obolibrary.org/obo/cpo#cpo_0000005"/>
        <obo:IAO_0000115>a cognitive factor that affects the level of influence of an implementation strategy before a mechanism acts on the situation</obo:IAO_0000115>
        <obo:IAO_0000116>the authors of the cited source are unclear concerning the definitive difference between &apos;cognitive&apos; and &apos;organizational&apos; moderators except in the diagrams on page 3. The indicates a temporal difference between the two, which has been represented here.</obo:IAO_0000116>
        <obo:IAO_0000119>Lewis CC, Klasnja P, Powell BJ, Lyon AR, Tuzzio L, Jones S, et al. From Classification to Causality: Advancing Understanding of Mechanisms of Change in Implementation Science. Front Public Health [Internet]. 2018 [cited 2018 Jun 6];6. Available from: https://www.frontiersin.org/articles/10.3389/fpubh.2018.00136/full</obo:IAO_0000119>
        <rdfs:label xml:lang="en">cognitive moderator</rdfs:label>
    </owl:Class>
    


    <!-- http://purl.obolibrary.org/obo/cpo#cpo_0000009 -->

    <owl:Class rdf:about="http://purl.obolibrary.org/obo/cpo#cpo_0000009">
        <rdfs:subClassOf rdf:resource="http://purl.obolibrary.org/obo/cpo#cpo_0000005"/>
        <obo:IAO_0000115>an organizational factor that affects the level of influence of an implementation strategy after, or simultaneously with, a mechanism that acts on the situation</obo:IAO_0000115>
        <obo:IAO_0000119>Lewis CC, Klasnja P, Powell BJ, Lyon AR, Tuzzio L, Jones S, et al. From Classification to Causality: Advancing Understanding of Mechanisms of Change in Implementation Science. Front Public Health [Internet]. 2018 [cited 2018 Jun 6];6. Available from: https://www.frontiersin.org/articles/10.3389/fpubh.2018.00136/full</obo:IAO_0000119>
        <rdfs:label xml:lang="en">organizational moderator</rdfs:label>
    </owl:Class>
    


    <!-- http://purl.obolibrary.org/obo/cpo#cpo_0000010 -->

    <owl:Class rdf:about="http://purl.obolibrary.org/obo/cpo#cpo_0000010">
        <rdfs:subClassOf rdf:resource="http://purl.obolibrary.org/obo/BFO_0000031"/>
        <obo:IAO_0000115>a purposeful procedure to achieve a specified outcome</obo:IAO_0000115>
        <obo:IAO_0000116>Many of the subclasses for this term were taken as-is from “EPOC Taxonomy | Cochrane Effective Practice and Organisation of Care.” The complete taxomony structure was not taken. Need to revisit.</obo:IAO_0000116>
        <obo:IAO_0000116>Secondary definition: the methods or techniques used to enhance the adoption, implementation, and sustainability of a program or practice.

From: Pai et al., “Strategies to Enhance Venous Thromboprophylaxis in Hospitalized Medical Patients (SENTRY).”</obo:IAO_0000116>
        <obo:IAO_0000116>this term is a good candidate for IAO &apos;Planned Process&apos;</obo:IAO_0000116>
        <obo:IAO_0000119>Mazza et al., “Refining a Taxonomy for Guideline Implementation.”</obo:IAO_0000119>
        <rdfs:label xml:lang="en">implementation strategy</rdfs:label>
    </owl:Class>
    


    <!-- http://purl.obolibrary.org/obo/cpo#cpo_0000011 -->

    <owl:Class rdf:about="http://purl.obolibrary.org/obo/cpo#cpo_0000011">
        <rdfs:subClassOf rdf:resource="http://purl.obolibrary.org/obo/BFO_0000015"/>
        <obo:IAO_0000115>the process of intervening on people, groups, entities or objects in an experimental study</obo:IAO_0000115>
        <obo:IAO_0000116>In controlled trials, the word is sometimes used to describe the regimens in all comparison groups, including placebo and no-treatment arms</obo:IAO_0000116>
        <obo:IAO_0000119>“Glossary | Cochrane Community.”</obo:IAO_0000119>
        <rdfs:label xml:lang="en">intervention</rdfs:label>
    </owl:Class>
    


    <!-- http://purl.obolibrary.org/obo/cpo#cpo_0000013 -->

    <owl:Class rdf:about="http://purl.obolibrary.org/obo/cpo#cpo_0000013">
        <rdfs:subClassOf rdf:resource="http://purl.obolibrary.org/obo/BFO_0000031"/>
        <obo:IAO_0000115>the conditions and circumstances that are relevant to the application of an intervention</obo:IAO_0000115>
        <obo:IAO_0000116>for example the setting (in hospital, at home, in the air); the time (working day, holiday, night-time); type of practice (primary, secondary, tertiary care; private practice, insurance practice, charity); whether routine or emergency</obo:IAO_0000116>
        <obo:IAO_0000119>“Glossary | Cochrane Community.”</obo:IAO_0000119>
        <rdfs:label xml:lang="en">context</rdfs:label>
    </owl:Class>
    


    <!-- http://purl.obolibrary.org/obo/cpo#cpo_0000014 -->

    <owl:Class rdf:about="http://purl.obolibrary.org/obo/cpo#cpo_0000014">
        <rdfs:subClassOf rdf:resource="http://purl.obolibrary.org/obo/BFO_0000020"/>
        <obo:IAO_0000115>the extent to which a specific intervention, when used under ordinary circumstances, does what it is intended to do</obo:IAO_0000115>
        <obo:IAO_0000119>“Glossary | Cochrane Community.”</obo:IAO_0000119>
        <rdfs:label xml:lang="en">effectiveness</rdfs:label>
    </owl:Class>
    


    <!-- http://purl.obolibrary.org/obo/cpo#cpo_0000016 -->

    <owl:Class rdf:about="http://purl.obolibrary.org/obo/cpo#cpo_0000016">
        <rdfs:subClassOf rdf:resource="http://purl.obolibrary.org/obo/BFO_0000031"/>
        <obo:IAO_0000115>a component of a recipient&apos;s status after an intervention has been applied that is used to assess the effectiveness of an intervention</obo:IAO_0000115>
        <obo:IAO_0000119>“Glossary | Cochrane Community.”</obo:IAO_0000119>
        <rdfs:label xml:lang="en">outcome</rdfs:label>
    </owl:Class>
    


    <!-- http://purl.obolibrary.org/obo/cpo#cpo_0000017 -->

    <owl:Class rdf:about="http://purl.obolibrary.org/obo/cpo#cpo_0000017">
        <rdfs:subClassOf rdf:resource="http://purl.obolibrary.org/obo/cpo#cpo_0000010"/>
        <obo:IAO_0000115>strategies to change organisational culture</obo:IAO_0000115>
        <obo:IAO_0000119>“EPOC Taxonomy | Cochrane Effective Practice and Organisation of Care.”</obo:IAO_0000119>
        <rdfs:label xml:lang="en">organisational culture</rdfs:label>
    </owl:Class>
    


    <!-- http://purl.obolibrary.org/obo/cpo#cpo_0000018 -->

    <owl:Class rdf:about="http://purl.obolibrary.org/obo/cpo#cpo_0000018">
        <rdfs:subClassOf rdf:resource="http://purl.obolibrary.org/obo/cpo#cpo_0000010"/>
        <obo:IAO_0000115>a summary of health workers’ performance over a specified period of time, given to them in a written electronic or verbal format. The summary may include recommendations for clinical action</obo:IAO_0000115>
        <obo:IAO_0000119>“EPOC Taxonomy | Cochrane Effective Practice and Organisation of Care.”</obo:IAO_0000119>
        <rdfs:label xml:lang="en">audit and feedback</rdfs:label>
    </owl:Class>
    


    <!-- http://purl.obolibrary.org/obo/cpo#cpo_0000019 -->

    <owl:Class rdf:about="http://purl.obolibrary.org/obo/cpo#cpo_0000019">
        <rdfs:subClassOf rdf:resource="http://purl.obolibrary.org/obo/cpo#cpo_0000010"/>
        <obo:IAO_0000115>monitoring of health services by individuals or healthcare organisations, for example by comparing with an external standard</obo:IAO_0000115>
        <obo:IAO_0000115>“EPOC Taxonomy | Cochrane Effective Practice and Organisation of Care.”</obo:IAO_0000115>
        <rdfs:label xml:lang="en">monitoring the performance of the delivery of healthcare</rdfs:label>
    </owl:Class>
    


    <!-- http://purl.obolibrary.org/obo/cpo#cpo_0000020 -->

    <owl:Class rdf:about="http://purl.obolibrary.org/obo/cpo#cpo_0000020">
        <rdfs:subClassOf rdf:resource="http://purl.obolibrary.org/obo/cpo#cpo_0000010"/>
        <obo:IAO_0000115>An iterative process to review and improve care that includes involvement of healthcare teams, analysis of a process or system, a structured process improvement method or problem solving approach, and use of data analysis to assess changes</obo:IAO_0000115>
        <obo:IAO_0000115>“EPOC Taxonomy | Cochrane Effective Practice and Organisation of Care.”</obo:IAO_0000115>
        <rdfs:label xml:lang="en">continuous quality improvement</rdfs:label>
    </owl:Class>
    


    <!-- http://purl.obolibrary.org/obo/cpo#cpo_0000021 -->

    <owl:Class rdf:about="http://purl.obolibrary.org/obo/cpo#cpo_0000021">
        <rdfs:subClassOf rdf:resource="http://purl.obolibrary.org/obo/cpo#cpo_0000010"/>
        <obo:IAO_0000115>interventions to change practice that are selected based on an assessment of barriers to change, for example through interviews or surveys</obo:IAO_0000115>
        <obo:IAO_0000119>“EPOC Taxonomy | Cochrane Effective Practice and Organisation of Care.”</obo:IAO_0000119>
        <rdfs:label xml:lang="en">tailored interventions</rdfs:label>
    </owl:Class>
    


    <!-- http://purl.obolibrary.org/obo/cpo#cpo_0000023 -->

    <owl:Class rdf:about="http://purl.obolibrary.org/obo/cpo#cpo_0000023">
        <rdfs:subClassOf rdf:resource="http://purl.obolibrary.org/obo/cpo#cpo_0000001"/>
        <obo:IAO_0000115>a mechanism that affects the ability to focus selectively on aspects of the environment</obo:IAO_0000115>
        <obo:IAO_0000119>Cane J, O’Connor D, Michie S. Validation of the theoretical domains framework for use in behaviour change and implementation research. Implementation Science. 2012 Apr 24;7:37.</obo:IAO_0000119>
        <rdfs:label xml:lang="en">act on attention</rdfs:label>
    </owl:Class>
    


    <!-- http://purl.obolibrary.org/obo/cpo#cpo_0000024 -->

    <owl:Class rdf:about="http://purl.obolibrary.org/obo/cpo#cpo_0000024">
        <rdfs:subClassOf rdf:resource="http://purl.obolibrary.org/obo/cpo#cpo_0000001"/>
        <obo:IAO_0000115>a mechanism that affects acceptance of the truth, reality, or validity about an ability, talent, or facility that a person can put to constructive use</obo:IAO_0000115>
        <obo:IAO_0000119>Cane J, O’Connor D, Michie S. Validation of the theoretical domains framework for use in behaviour change and implementation research. Implementation Science. 2012 Apr 24;7:37.</obo:IAO_0000119>
        <obo:IAO_0000119>Kolehmainen N, Francis JJ. Specifying content and mechanisms of change in interventions to change professionals’ practice: an illustration from the Good Goals study in occupational therapy. Implementation Science. 2012 Oct 18;7:100.</obo:IAO_0000119>
        <rdfs:label xml:lang="en">act on belief about capabilities</rdfs:label>
    </owl:Class>
    


    <!-- http://purl.obolibrary.org/obo/cpo#cpo_0000025 -->

    <owl:Class rdf:about="http://purl.obolibrary.org/obo/cpo#cpo_0000025">
        <rdfs:subClassOf rdf:resource="http://purl.obolibrary.org/obo/cpo#cpo_0000001"/>
        <obo:IAO_0000115>a mechanism that affects a complex reaction pattern, involving experiential, behavioural, and physiological elements, by which the individual attempts to deal with a personally significant matter or event</obo:IAO_0000115>
        <obo:IAO_0000119>Cane J, O’Connor D, Michie S. Validation of the theoretical domains framework for use in behaviour change and implementation research. Implementation Science. 2012 Apr 24;7:37.</obo:IAO_0000119>
        <obo:IAO_0000119>Kolehmainen N, Francis JJ. Specifying content and mechanisms of change in interventions to change professionals’ practice: an illustration from the Good Goals study in occupational therapy. Implementation Science. 2012 Oct 18;7:100.</obo:IAO_0000119>
        <rdfs:label xml:lang="en">act on emotion</rdfs:label>
    </owl:Class>
    


    <!-- http://purl.obolibrary.org/obo/cpo#cpo_0000029 -->

    <owl:Class rdf:about="http://purl.obolibrary.org/obo/cpo#cpo_0000029">
        <rdfs:subClassOf rdf:resource="http://purl.obolibrary.org/obo/BFO_0000031"/>
        <obo:IAO_0000115>the structure of the relation of variables and outcomes in a specific context</obo:IAO_0000115>
        <obo:IAO_0000116>a casual pathway is a set of features &quot;of the mechanistic processes
through which implementation strategies operate&quot; (Lewis 2018).</obo:IAO_0000116>
        <obo:IAO_0000119>Lewis CC, Klasnja P, Powell BJ, Lyon AR, Tuzzio L, Jones S, et al. From Classification to Causality: Advancing Understanding of Mechanisms of Change in Implementation Science. Front Public Health [Internet]. 2018 [cited 2018 Jun 6];6. Available from: https://www.frontiersin.org/articles/10.3389/fpubh.2018.00136/full</obo:IAO_0000119>
        <rdfs:label xml:lang="en">casual pathway</rdfs:label>
    </owl:Class>
    


    <!-- http://purl.obolibrary.org/obo/cpo#cpo_0000030 -->

    <owl:Class rdf:about="http://purl.obolibrary.org/obo/cpo#cpo_0000030">
        <rdfs:subClassOf rdf:resource="http://purl.obolibrary.org/obo/cpo#cpo_0000002"/>
        <obo:IAO_0000115>a precondition that allows for the possibility of a mechanism to act</obo:IAO_0000115>
        <obo:IAO_0000119>Lewis CC, Klasnja P, Powell BJ, Lyon AR, Tuzzio L, Jones S, et al. From Classification to Causality: Advancing Understanding of Mechanisms of Change in Implementation Science. Front Public Health [Internet]. 2018 [cited 2018 Jun 6];6. Available from: https://www.frontiersin.org/articles/10.3389/fpubh.2018.00136/full</obo:IAO_0000119>
        <rdfs:label xml:lang="en">precondition for mechanism of activation</rdfs:label>
    </owl:Class>
    


    <!-- http://purl.obolibrary.org/obo/cpo#cpo_0000031 -->

    <owl:Class rdf:about="http://purl.obolibrary.org/obo/cpo#cpo_0000031">
        <rdfs:subClassOf rdf:resource="http://purl.obolibrary.org/obo/cpo#cpo_0000002"/>
        <obo:IAO_0000115>a precondition that allows for the possibility of a proximal outcome</obo:IAO_0000115>
        <obo:IAO_0000119>Lewis CC, Klasnja P, Powell BJ, Lyon AR, Tuzzio L, Jones S, et al. From Classification to Causality: Advancing Understanding of Mechanisms of Change in Implementation Science. Front Public Health [Internet]. 2018 [cited 2018 Jun 6];6. Available from: https://www.frontiersin.org/articles/10.3389/fpubh.2018.00136/full</obo:IAO_0000119>
        <rdfs:label xml:lang="en">precondition for proximal outcome</rdfs:label>
    </owl:Class>
    


    <!-- http://purl.obolibrary.org/obo/cpo#cpo_0000032 -->

    <owl:Class rdf:about="http://purl.obolibrary.org/obo/cpo#cpo_0000032">
        <rdfs:subClassOf rdf:resource="http://purl.obolibrary.org/obo/cpo#cpo_0000001"/>
        <obo:IAO_0000115>a mechanism that affects mental representations of outcomes or end states that an individual wants to achieve</obo:IAO_0000115>
        <obo:IAO_0000119>Cane J, O’Connor D, Michie S. Validation of the theoretical domains framework for use in behaviour change and implementation research. Implementation Science. 2012 Apr 24;7:37.</obo:IAO_0000119>
        <rdfs:label xml:lang="en">act on goal</rdfs:label>
    </owl:Class>
    


    <!-- http://purl.obolibrary.org/obo/cpo#cpo_0000033 -->

    <owl:Class rdf:about="http://purl.obolibrary.org/obo/cpo#cpo_0000033">
        <rdfs:subClassOf rdf:resource="http://purl.obolibrary.org/obo/cpo#cpo_0000001"/>
        <obo:IAO_0000115>a mechanism that affects an awareness of the existence of something</obo:IAO_0000115>
        <obo:IAO_0000119>Cane J, O’Connor D, Michie S. Validation of the theoretical domains framework for use in behaviour change and implementation research. Implementation Science. 2012 Apr 24;7:37.</obo:IAO_0000119>
        <rdfs:label xml:lang="en">act on knowledge</rdfs:label>
    </owl:Class>
    


    <!-- http://purl.obolibrary.org/obo/cpo#cpo_0000034 -->

    <owl:Class rdf:about="http://purl.obolibrary.org/obo/cpo#cpo_0000034">
        <rdfs:subClassOf rdf:resource="http://purl.obolibrary.org/obo/cpo#cpo_0000001"/>
        <obo:IAO_0000115>a mechanism that affects a conscious decision to perform a behaviour or a resolve to act in a certain way</obo:IAO_0000115>
        <obo:IAO_0000116>This was adapted from the category &apos;intention&apos; in the cited source. The authors list &apos;intrinic motivation&apos; under the category of intention. This needed to be revisited.</obo:IAO_0000116>
        <obo:IAO_0000119>Cane J, O’Connor D, Michie S. Validation of the theoretical domains framework for use in behaviour change and implementation research. Implementation Science. 2012 Apr 24;7:37.</obo:IAO_0000119>
        <rdfs:label xml:lang="en">act on motivation</rdfs:label>
    </owl:Class>
    


    <!-- http://purl.obolibrary.org/obo/cpo#cpo_0000035 -->

    <owl:Class rdf:about="http://purl.obolibrary.org/obo/cpo#cpo_0000035">
        <rdfs:subClassOf rdf:resource="http://purl.obolibrary.org/obo/cpo#cpo_0000008"/>
        <obo:IAO_0000115>a sensitivity of the intended recipient of an intevention towards gain and pleasure</obo:IAO_0000115>
        <obo:IAO_0000119>source needed</obo:IAO_0000119>
        <rdfs:label xml:lang="en">promotion focus</rdfs:label>
    </owl:Class>
    


    <!-- http://purl.obolibrary.org/obo/cpo#cpo_0000036 -->

    <owl:Class rdf:about="http://purl.obolibrary.org/obo/cpo#cpo_0000036">
        <rdfs:subClassOf rdf:resource="http://purl.obolibrary.org/obo/cpo#cpo_0000008"/>
        <obo:IAO_0000115>a sensitivity of the intended recipient of an intevention towards loss and avoidance of pain</obo:IAO_0000115>
        <obo:IAO_0000119>source needed</obo:IAO_0000119>
        <rdfs:label xml:lang="en">prevention focus</rdfs:label>
    </owl:Class>
    


    <!-- http://purl.obolibrary.org/obo/cpo#cpo_0000037 -->

    <owl:Class rdf:about="http://purl.obolibrary.org/obo/cpo#cpo_0000037">
        <rdfs:subClassOf rdf:resource="http://purl.obolibrary.org/obo/cpo#cpo_0000039"/>
        <obo:IAO_0000115>a method of presenting information that is intended to affect an intended reciepients&apos;s perception of gain or opporunity</obo:IAO_0000115>
        <obo:IAO_0000119>source needed</obo:IAO_0000119>
        <rdfs:label xml:lang="en">promotion framing</rdfs:label>
    </owl:Class>
    


    <!-- http://purl.obolibrary.org/obo/cpo#cpo_0000038 -->

    <owl:Class rdf:about="http://purl.obolibrary.org/obo/cpo#cpo_0000038">
        <rdfs:subClassOf rdf:resource="http://purl.obolibrary.org/obo/cpo#cpo_0000039"/>
        <obo:IAO_0000115>a method of presenting information that is intended to affect an intended reciepients&apos;s perception of loss or risk</obo:IAO_0000115>
        <obo:IAO_0000119>source needed</obo:IAO_0000119>
        <rdfs:label xml:lang="en">prevention framing</rdfs:label>
    </owl:Class>
    


    <!-- http://purl.obolibrary.org/obo/cpo#cpo_0000039 -->

    <owl:Class rdf:about="http://purl.obolibrary.org/obo/cpo#cpo_0000039">
        <rdfs:subClassOf rdf:resource="http://purl.obolibrary.org/obo/cpo#cpo_0000009"/>
        <obo:IAO_0000115>a method of presenting information that is intended to affect the influence of an implementation strategy</obo:IAO_0000115>
        <obo:IAO_0000119>source needed</obo:IAO_0000119>
        <rdfs:label xml:lang="en">message framing</rdfs:label>
    </owl:Class>
    


    <!-- http://purl.obolibrary.org/obo/cpo#cpo_0000040 -->

    <owl:Class rdf:about="http://purl.obolibrary.org/obo/cpo#cpo_0000040">
        <rdfs:subClassOf rdf:resource="http://purl.obolibrary.org/obo/cpo#cpo_0000030"/>
        <obo:IAO_0000115>def needed</obo:IAO_0000115>
        <rdfs:label xml:lang="en">performance precondition</rdfs:label>
    </owl:Class>
    


    <!-- http://purl.obolibrary.org/obo/cpo#cpo_0000041 -->

    <owl:Class rdf:about="http://purl.obolibrary.org/obo/cpo#cpo_0000041">
        <rdfs:subClassOf rdf:resource="http://purl.obolibrary.org/obo/cpo#cpo_0000040"/>
        <obo:IAO_0000115>def needed</obo:IAO_0000115>
        <rdfs:label xml:lang="en">high performance - downward trend</rdfs:label>
    </owl:Class>
    


    <!-- http://purl.obolibrary.org/obo/cpo#cpo_0000042 -->

    <owl:Class rdf:about="http://purl.obolibrary.org/obo/cpo#cpo_0000042">
        <rdfs:subClassOf rdf:resource="http://purl.obolibrary.org/obo/cpo#cpo_0000040"/>
        <obo:IAO_0000115>def needed</obo:IAO_0000115>
        <rdfs:label xml:lang="en">high performance - stable</rdfs:label>
    </owl:Class>
    


    <!-- http://purl.obolibrary.org/obo/cpo#cpo_0000043 -->

    <owl:Class rdf:about="http://purl.obolibrary.org/obo/cpo#cpo_0000043">
        <rdfs:subClassOf rdf:resource="http://purl.obolibrary.org/obo/cpo#cpo_0000040"/>
        <obo:IAO_0000115>def needed</obo:IAO_0000115>
        <rdfs:label xml:lang="en">high performance - upward trend</rdfs:label>
    </owl:Class>
    


    <!-- http://purl.obolibrary.org/obo/cpo#cpo_0000044 -->

    <owl:Class rdf:about="http://purl.obolibrary.org/obo/cpo#cpo_0000044">
        <rdfs:subClassOf rdf:resource="http://purl.obolibrary.org/obo/cpo#cpo_0000040"/>
        <obo:IAO_0000115>def needed</obo:IAO_0000115>
        <rdfs:label xml:lang="en">low performance - downward trend</rdfs:label>
    </owl:Class>
    


    <!-- http://purl.obolibrary.org/obo/cpo#cpo_0000045 -->

    <owl:Class rdf:about="http://purl.obolibrary.org/obo/cpo#cpo_0000045">
        <rdfs:subClassOf rdf:resource="http://purl.obolibrary.org/obo/cpo#cpo_0000040"/>
        <obo:IAO_0000115>def needed</obo:IAO_0000115>
        <rdfs:label xml:lang="en">low performance - stable</rdfs:label>
    </owl:Class>
    


    <!-- http://purl.obolibrary.org/obo/cpo#cpo_0000046 -->

    <owl:Class rdf:about="http://purl.obolibrary.org/obo/cpo#cpo_0000046">
        <rdfs:subClassOf rdf:resource="http://purl.obolibrary.org/obo/cpo#cpo_0000040"/>
        <obo:IAO_0000115>def needed</obo:IAO_0000115>
        <rdfs:label xml:lang="en">low performance - upward trend</rdfs:label>
    </owl:Class>
    


    <!-- http://purl.obolibrary.org/obo/cpo#cpo_0000047 -->

    <owl:Class rdf:about="http://purl.obolibrary.org/obo/cpo#cpo_0000047">
        <rdfs:subClassOf rdf:resource="http://purl.obolibrary.org/obo/cpo#cpo_0000040"/>
        <rdfs:label xml:lang="en">top performer</rdfs:label>
    </owl:Class>
</rdf:RDF>



<!-- Generated by the OWL API (version 4.2.8.20170104-2310) https://github.com/owlcs/owlapi -->

